src/parser/FStarC.Parser.AST.Diff.fst
@@ -16,7 +16,6 @@
    Authors: N. Swamy and Copilot
 *)
 module FStarC.Parser.AST.Diff
-#push-options "--MLish --MLish_effect FStarC.Effect"
 
 open FStarC
 open FStarC.Effect
@@ -24,16 +23,20 @@ open FStarC.Ident
 open FStarC.Const
 open FStarC.Parser.AST
 
-let eq_ident (i1 i2:ident) =
+private let ( &&& ) (a b : bool) : bool = a && b
+
+let eq_ident (i1 i2:ident) : ML bool =
   Ident.ident_equals i1 i2
 
-let eq_list (f: 'a -> 'a -> bool) (t1 t2:list 'a)
-  : bool
-  = List.length t1 = List.length t2 &&
-    List.forall2 f t1 t2
+let rec eq_list (f: 'a -> 'a -> ML bool) (t1 t2:list 'a)
+  : ML bool
+  = match t1, t2 with
+    | [], [] -> true
+    | x1::xs1, x2::xs2 -> if f x1 x2 then eq_list f xs1 xs2 else false
+    | _ -> false
 
-let eq_option (f: 'a -> 'a -> bool) (t1 t2:option 'a)
-  : bool
+let eq_option (f: 'a -> 'a -> ML bool) (t1 t2:option 'a)
+  : ML bool
   = match t1, t2 with
     | None, None -> true
     | Some t1, Some t2 -> f t1 t2
@@ -42,12 +45,12 @@ let eq_option (f: 'a -> 'a -> bool) (t1 t2:option 'a)
 //
 // TODO: There is an eq_const in FStarC.Const.fst, can we use that?
 //
-let eq_sconst (c1 c2: sconst) : bool =
+let eq_sconst (c1 c2: sconst) : ML bool =
     match c1, c2 with
     | Const_effect, Const_effect -> true
     | Const_unit, Const_unit -> true
     | Const_bool b1, Const_bool b2 -> b1 = b2
-    | Const_int (s1, sw1), Const_int (s2, sw2) -> s1=s2 && sw1=sw2
+    | Const_int (s1, sw1), Const_int (s2, sw2) -> s1=s2 &&& sw1=sw2
     | Const_char c1, Const_char c2 -> c1 = c2
     | Const_string (s1, _), Const_string (s2, _) -> s1 = s2
     | Const_real s1, Const_real s2 -> s1 = s2
@@ -57,20 +60,22 @@ let eq_sconst (c1 c2: sconst) : bool =
     | _ -> false
 
 let rec eq_term (t1 t2:term)
-  : bool
+  : ML bool
   = eq_term' t1.tm t2.tm
 
 and eq_terms (t1 t2:list term)
-  : bool
+  : ML bool
   = eq_list eq_term t1 t2
 
 and eq_arg (t1 t2 : (term & imp))
+  : ML bool
   = let t1, a1 = t1 in
     let t2, a2 = t2 in
-    eq_term t1 t2 &&
+    eq_term t1 t2 &&&
     eq_imp a1 a2
 
 and eq_imp (i1 i2: imp)
+  : ML bool
   = match i1, i2 with
     | Hash, Hash
     | UnivApp, UnivApp
@@ -81,10 +86,10 @@ and eq_imp (i1 i2: imp)
     | _ -> false
 
 and eq_args (t1 t2: list (term & imp))
-  : bool
+  : ML bool
   = eq_list eq_arg t1 t2
 
-and eq_arg_qualifier (arg_qualifier1:arg_qualifier) (arg_qualifier2:arg_qualifier) : bool =
+and eq_arg_qualifier (arg_qualifier1:arg_qualifier) (arg_qualifier2:arg_qualifier) : ML bool =
   match arg_qualifier1, arg_qualifier2 with
   | Implicit, Implicit -> true
   | Equality, Equality -> true
@@ -93,25 +98,25 @@ and eq_arg_qualifier (arg_qualifier1:arg_qualifier) (arg_qualifier2:arg_qualifie
   | _ -> false
 
 and eq_pattern (p1 p2:pattern)
-  : bool
+  : ML bool
   = eq_pattern' p1.pat p2.pat
 
-and eq_aqual a1 a2 = eq_option eq_arg_qualifier a1 a2
+and eq_aqual a1 a2 : ML bool = eq_option eq_arg_qualifier a1 a2
 
 and eq_pattern' (p1 p2:pattern')
-  : bool
+  : ML bool
   = match p1, p2 with
     | PatWild(q1, a1), PatWild(q2, a2) ->
-      eq_aqual q1 q2 &&
+      eq_aqual q1 q2 &&&
       eq_terms a1 a2
     | PatConst s1, PatConst s2 ->
       eq_sconst s1 s2
     | PatApp (p1, ps1), PatApp(p2, ps2) ->
-      eq_pattern p1 p2 &&
+      eq_pattern p1 p2 &&&
       eq_list eq_pattern ps1 ps2
     | PatVar (i1, aq1, as1), PatVar(i2, aq2, as2) ->
-      Ident.ident_equals i1 i2 &&
-      eq_aqual aq1 aq2 &&
+      Ident.ident_equals i1 i2 &&&
+      eq_aqual aq1 aq2 &&&
       eq_terms as1 as2
     | PatName l1, PatName l2 ->
       Ident.lid_equals l1 l2
@@ -119,16 +124,16 @@ and eq_pattern' (p1 p2:pattern')
     | PatList ps1, PatList ps2 ->
       eq_list eq_pattern ps1 ps2
     | PatTuple(ps1, b1), PatTuple(ps2, b2) ->
-      eq_list eq_pattern ps1 ps2 &&
+      eq_list eq_pattern ps1 ps2 &&&
       b1 = b2
     | PatRecord ps1, PatRecord ps2 ->
       eq_list (fun (l1, p1) (l2, p2) ->
-                 Ident.lid_equals l1 l2 &&
+                 Ident.lid_equals l1 l2 &&&
                  eq_pattern p1 p2)
               ps1 ps2
     | PatAscribed (p1, (t1, topt1)), PatAscribed (p2, (t2, topt2)) ->
-      eq_pattern p1 p2 &&
-      eq_term t1 t2 &&
+      eq_pattern p1 p2 &&&
+      eq_term t1 t2 &&&
       eq_option eq_term topt1 topt2
     | PatOp i1, PatOp i2 ->
       eq_ident i1 i2
@@ -139,12 +144,12 @@ and eq_pattern' (p1 p2:pattern')
     | _ -> false
 
 and eq_term' (t1 t2:term')
-  : bool
+  : ML bool
   = match t1, t2 with
     | Wild, Wild -> true
     | Const s1, Const s2 -> eq_const s1 s2
     | Op (i1, ts1), Op (i2, ts2) ->
-      eq_ident i1 i2 &&
+      eq_ident i1 i2 &&&
       eq_terms ts1 ts2
     | Uvar i1, Uvar i2 ->
       eq_ident i1 i2
@@ -152,80 +157,80 @@ and eq_term' (t1 t2:term')
     | Name l1, Name l2 ->
       Ident.lid_equals l1 l2
     | Projector (l1, i1), Projector (l2, i2) ->
-      Ident.lid_equals l1 l2 &&
+      Ident.lid_equals l1 l2 &&&
       Ident.ident_equals i1 i2
     | Construct (l1, args1), Construct (l2, args2) ->
-      Ident.lid_equals l1 l2 &&
+      Ident.lid_equals l1 l2 &&&
       eq_args args1 args2
     | Function (brs1, _r1), Function (brs2, _r2) ->
       eq_list eq_branch brs1 brs2
     | Abs (ps1, t1), Abs (ps2, t2) ->
-      eq_list eq_pattern ps1 ps2 &&
+      eq_list eq_pattern ps1 ps2 &&&
       eq_term t1 t2
     | App (h1, t1, i1), App(h2, t2, i2) ->
-      eq_term h1 h2 &&
-      eq_term t1 t2 &&
+      eq_term h1 h2 &&&
+      eq_term t1 t2 &&&
       eq_imp i1 i2
     | Let (lq1, defs1, t1), Let (lq2, defs2, t2) ->
-      lq1=lq2 &&
+      lq1=lq2 &&&
       eq_list (fun (o1, (p1, t1)) (o2, (p2, t2)) ->
-                 eq_option eq_terms o1 o2 &&
-                 eq_pattern p1 p2 &&
+                 eq_option eq_terms o1 o2 &&&
+                 eq_pattern p1 p2 &&&
                  eq_term t1 t2)
-              defs1 defs2 &&
+              defs1 defs2 &&&
       eq_term t1 t2
     | LetOperator (defs1, t1), LetOperator (defs2, t2) ->
       eq_list (fun (i1, ps1, t1) (i2, ps2, t2) ->
-                 eq_ident i1 i2 &&
-                 eq_pattern ps1 ps2 &&
+                 eq_ident i1 i2 &&&
+                 eq_pattern ps1 ps2 &&&
                  eq_term t1 t2)
-              defs1 defs2 &&
+              defs1 defs2 &&&
       eq_term t1 t2
     | LetOpen (l1, t1), LetOpen (l2, t2) ->
-      Ident.lid_equals l1 l2 &&
+      Ident.lid_equals l1 l2 &&&
       eq_term t1 t2
     // compare all the remaining cases of terms starting with LetOperator
     | LetOpenRecord (t1, t2, t3), LetOpenRecord (t4, t5, t6) ->
-      eq_term t1 t4 &&
-      eq_term t2 t5 &&
+      eq_term t1 t4 &&&
+      eq_term t2 t5 &&&
       eq_term t3 t6
     | Seq (t1, t2), Seq (t3, t4) ->
-      eq_term t1 t3 &&
+      eq_term t1 t3 &&&
       eq_term t2 t4
     | Bind (i1, t1, t2), Bind (i2, t3, t4) ->
-      Ident.ident_equals i1 i2 &&
-      eq_term t1 t3 &&
+      Ident.ident_equals i1 i2 &&&
+      eq_term t1 t3 &&&
       eq_term t2 t4
     | If (t1, i1, mra1, t2, t3), If (t4, i2, mra2, t5, t6) ->
-      eq_term t1 t4 &&
-      eq_option eq_ident i1 i2 &&
-      eq_option eq_match_returns_annotation mra1 mra2 &&
-      eq_term t2 t5 &&
+      eq_term t1 t4 &&&
+      eq_option eq_ident i1 i2 &&&
+      eq_option eq_match_returns_annotation mra1 mra2 &&&
+      eq_term t2 t5 &&&
       eq_term t3 t6
     | Match (t1, i1, mra1, bs1), Match (t2, i2, mra2, bs2) ->
-      eq_term t1 t2 &&
-      eq_option eq_ident i1 i2 &&
-      eq_option eq_match_returns_annotation mra1 mra2 &&
+      eq_term t1 t2 &&&
+      eq_option eq_ident i1 i2 &&&
+      eq_option eq_match_returns_annotation mra1 mra2 &&&
       eq_list eq_branch bs1 bs2
     | TryWith (t1, bs1), TryWith (t2, bs2) ->
-      eq_term t1 t2 &&
+      eq_term t1 t2 &&&
       eq_list eq_branch bs1 bs2
     | Ascribed (t1, t2, topt1, b1), Ascribed (t3, t4, topt2, b2) ->
-      eq_term t1 t3 &&
-      eq_term t2 t4 &&
-      eq_option eq_term topt1 topt2 &&
+      eq_term t1 t3 &&&
+      eq_term t2 t4 &&&
+      eq_option eq_term topt1 topt2 &&&
       b1 = b2
     | Record (topt1, fs1), Record (topt2, fs2) ->
-      eq_option eq_term topt1 topt2 &&
+      eq_option eq_term topt1 topt2 &&&
       eq_list (fun (l1, t1) (l2, t2) ->
-                 Ident.lid_equals l1 l2 &&
+                 Ident.lid_equals l1 l2 &&&
                  eq_term t1 t2)
               fs1 fs2
     | Project (t1, l1), Project (t2, l2) ->
-      eq_term t1 t2 &&
+      eq_term t1 t2 &&&
       Ident.lid_equals l1 l2
     | Product (bs1, t1), Product (bs2, t2) ->
-      eq_list eq_binder bs1 bs2 &&
+      eq_list eq_binder bs1 bs2 &&&
       eq_term t1 t2
     | Sum (bs1, t1), Sum (bs2, t2) ->
       eq_list (fun b1 b2 ->
@@ -237,35 +242,35 @@ and eq_term' (t1 t2:term')
                  | Inl _, Inr _
                  | Inr _, Inl _ ->
                    false)
-              bs1 bs2 &&
+              bs1 bs2 &&&
       eq_term t1 t2
     | QForall (bs1, ps1, t1), QForall (bs2, ps2, t2)
     | QExists (bs1, ps1, t1), QExists (bs2, ps2, t2) ->
       //ps1 and ps2 have type list ident * list (list term)
       // generate equality on ps1 p2
       let eq_ps (is1, ts1) (is2, ts2) =
-        eq_list eq_ident is1 is2 &&
+        eq_list eq_ident is1 is2 &&&
         eq_list (eq_list eq_term) ts1 ts2
       in
-      eq_list eq_binder bs1 bs2 &&
-      eq_ps ps1 ps2 &&
+      eq_list eq_binder bs1 bs2 &&&
+      eq_ps ps1 ps2 &&&
       eq_term t1 t2
     | QuantOp (i1, bs1, ps1, t1), QuantOp (i2, bs2, ps2, t2) ->
       let eq_ps (is1, ts1) (is2, ts2) =
-        eq_list eq_ident is1 is2 &&
+        eq_list eq_ident is1 is2 &&&
         eq_list (eq_list eq_term) ts1 ts2
       in
-      Ident.ident_equals i1 i2 &&
-      eq_list eq_binder bs1 bs2 &&
-      eq_ps ps1 ps2 &&
+      Ident.ident_equals i1 i2 &&&
+      eq_list eq_binder bs1 bs2 &&&
+      eq_ps ps1 ps2 &&&
       eq_term t1 t2
     // continue comparing all the remaining cases of terms, starting with Refine
     | Refine (t1, t2), Refine (t3, t4) ->
-      eq_binder t1 t3 &&
+      eq_binder t1 t3 &&&
       eq_term t2 t4
     // continue comparing all the remaining cases of terms, starting with NamedTyp
     | NamedTyp (i1, t1), NamedTyp (i2, t2) ->
-      eq_ident i1 i2 &&
+      eq_ident i1 i2 &&&
       eq_term t1 t2
     | Paren t1, Paren t2 ->
       eq_term t1 t2
@@ -276,13 +281,13 @@ and eq_term' (t1 t2:term')
     | LexList ts1, LexList ts2 ->
       eq_list eq_term ts1 ts2
     | WFOrder (t1, t2), WFOrder (t3, t4) ->
-      eq_term t1 t3 &&
+      eq_term t1 t3 &&&
       eq_term t2 t4
     | Decreases t1, Decreases t2 ->
       eq_term t1 t2
     | Labeled (t1, s1, b1), Labeled (t2, s2, b2) ->
-      eq_term t1 t2 &&
-      s1 = s2 &&
+      eq_term t1 t2 &&&
+      s1 = s2 &&&
       b1 = b2
     | Discrim l1, Discrim l2 ->
       Ident.lid_equals l1 l2
@@ -291,66 +296,66 @@ and eq_term' (t1 t2:term')
     | Antiquote t1, Antiquote t2 ->
       eq_term t1 t2
     | Quote (t1, k1), Quote (t2, k2) ->
-      eq_term t1 t2 &&
+      eq_term t1 t2 &&&
       k1 = k2
     | VQuote t1, VQuote t2 ->
       eq_term t1 t2
     | CalcProof (t1, t2, cs1), CalcProof (t3, t4, cs2) ->
-      eq_term t1 t3 &&
-      eq_term t2 t4 &&
+      eq_term t1 t3 &&&
+      eq_term t2 t4 &&&
       eq_list eq_calc_step cs1 cs2
     | IntroForall (bs1, t1, t2), IntroForall (bs2, t3, t4) ->
-      eq_list eq_binder bs1 bs2 &&
-      eq_term t1 t3 &&
+      eq_list eq_binder bs1 bs2 &&&
+      eq_term t1 t3 &&&
       eq_term t2 t4
     | IntroExists (bs1, t1, ts1, t2), IntroExists (bs2, t3, ts2, t4) ->
-      eq_list eq_binder bs1 bs2 &&
-      eq_term t1 t3 &&
-      eq_list eq_term ts1 ts2 &&
+      eq_list eq_binder bs1 bs2 &&&
+      eq_term t1 t3 &&&
+      eq_list eq_term ts1 ts2 &&&
       eq_term t2 t4
     | IntroImplies (t1, t2, b1, t3), IntroImplies (t4, t5, b2, t6) ->
-      eq_term t1 t4 &&
-      eq_term t2 t5 &&
-      eq_binder b1 b2 &&
+      eq_term t1 t4 &&&
+      eq_term t2 t5 &&&
+      eq_binder b1 b2 &&&
       eq_term t3 t6
     | IntroOr (b1, t1, t2, t3), IntroOr (b2, t4, t5, t6) ->
-      b1 = b2 &&
-      eq_term t1 t4 &&
-      eq_term t2 t5 &&
+      b1 = b2 &&&
+      eq_term t1 t4 &&&
+      eq_term t2 t5 &&&
       eq_term t3 t6
     | IntroAnd (t1, t2, t3, t4), IntroAnd (t5, t6, t7, t8) ->
-      eq_term t1 t5 &&
-      eq_term t2 t6 &&
-      eq_term t3 t7 &&
+      eq_term t1 t5 &&&
+      eq_term t2 t6 &&&
+      eq_term t3 t7 &&&
       eq_term t4 t8
     | ElimForall (bs1, t1, ts1), ElimForall (bs2, t2, ts2) ->
-      eq_list eq_binder bs1 bs2 &&
-      eq_term t1 t2 &&
+      eq_list eq_binder bs1 bs2 &&&
+      eq_term t1 t2 &&&
       eq_list eq_term ts1 ts2
     | ElimExists (bs1, t1, t2, b1, t3), ElimExists (bs2, t4, t5, b2, t6) ->
-      eq_list eq_binder bs1 bs2 &&
-      eq_term t1 t4 &&
-      eq_term t2 t5 &&
-      eq_binder b1 b2 &&
+      eq_list eq_binder bs1 bs2 &&&
+      eq_term t1 t4 &&&
+      eq_term t2 t5 &&&
+      eq_binder b1 b2 &&&
       eq_term t3 t6
     | ElimImplies (t1, t2, t3), ElimImplies (t4, t5, t6) ->
-      eq_term t1 t4 &&
-      eq_term t2 t5 &&
+      eq_term t1 t4 &&&
+      eq_term t2 t5 &&&
       eq_term t3 t6
     | ElimOr (t1, t2, t3, b1, t4, b2, t5), ElimOr (t6, t7, t8, b3, t9, b4, t10) ->
-      eq_term t1 t6 &&
-      eq_term t2 t7 &&
-      eq_term t3 t8 &&
-      eq_binder b1 b3 &&
-      eq_term t4 t9 &&
-      eq_binder b2 b4 &&
+      eq_term t1 t6 &&&
+      eq_term t2 t7 &&&
+      eq_term t3 t8 &&&
+      eq_binder b1 b3 &&&
+      eq_term t4 t9 &&&
+      eq_binder b2 b4 &&&
       eq_term t5 t10
     | ElimAnd (t1, t2, t3, b1, b2, t4), ElimAnd (t5, t6, t7, b3, b4, t8) ->
-      eq_term t1 t5 &&
-      eq_term t2 t6 &&
-      eq_term t3 t7 &&
-      eq_binder b1 b3 &&
-      eq_binder b2 b4 &&
+      eq_term t1 t5 &&&
+      eq_term t2 t6 &&&
+      eq_term t3 t7 &&&
+      eq_binder b1 b3 &&&
+      eq_binder b2 b4 &&&
       eq_term t4 t8
     | ListLiteral ts1, ListLiteral ts2 ->
       eq_list eq_term ts1 ts2
@@ -358,95 +363,101 @@ and eq_term' (t1 t2:term')
       eq_list eq_term ts1 ts2
     | _ -> false
 
-and eq_calc_step (CalcStep (t1, t2, t3)) (CalcStep (t4, t5, t6)) =
-    eq_term t1 t4 &&
-    eq_term t2 t5 &&
+and eq_calc_step (s1 s2: calc_step) : ML bool =
+    let CalcStep (t1, t2, t3) = s1 in
+    let CalcStep (t4, t5, t6) = s2 in
+    eq_term t1 t4 &&&
+    eq_term t2 t5 &&&
     eq_term t3 t6
 
-and eq_binder (b1 b2:binder) =
-  eq_binder' b1.b b2.b &&
-  eq_aqual b1.aqual b2.aqual &&
+and eq_binder (b1 b2:binder) : ML bool =
+  eq_binder' b1.b b2.b &&&
+  eq_aqual b1.aqual b2.aqual &&&
   eq_list eq_term b1.battributes b2.battributes
 
-and eq_binder' (b1 b2:binder') =
+and eq_binder' (b1 b2:binder') : ML bool =
   match b1, b2 with
   | Variable i1, Variable i2 -> eq_ident i1 i2
   | Annotated (i1, t1), Annotated (i2, t2) ->
-      eq_ident i1 i2 &&
+      eq_ident i1 i2 &&&
       eq_term t1 t2
   | NoName t1, NoName t2 ->
       eq_term t1 t2
   | _ -> false
 
-and eq_match_returns_annotation (i1, t1, b1) (i2, t2, b2) =
-    eq_option eq_ident i1 i2 &&
-    eq_term t1 t2 &&
+and eq_match_returns_annotation (a1 a2: (option ident & term & bool)) : ML bool =
+    let (i1, t1, b1) = a1 in
+    let (i2, t2, b2) = a2 in
+    eq_option eq_ident i1 i2 &&&
+    eq_term t1 t2 &&&
     b1 = b2
 
-and eq_branch (p1, o1, t1) (p2, o2, t2) =
-    eq_pattern p1 p2 &&
-    eq_option eq_term o1 o2 &&
+and eq_branch (br1 br2: (pattern & option term & term)) : ML bool =
+    let (p1, o1, t1) = br1 in
+    let (p2, o2, t2) = br2 in
+    eq_pattern p1 p2 &&&
+    eq_option eq_term o1 o2 &&&
     eq_term t1 t2
 
 
-let eq_tycon_record (t1 t2: tycon_record) =
+let eq_tycon_record (t1 t2: tycon_record) : ML bool =
   eq_list (fun (i1, a1, a2, t1) (i2, a3, a4, t2) ->
-    eq_ident i1 i2 &&
-    eq_aqual a1 a3 &&
-    eq_list eq_term a2 a4 &&
+    eq_ident i1 i2 &&&
+    eq_aqual a1 a3 &&&
+    eq_list eq_term a2 a4 &&&
     eq_term t1 t2) t1 t2
 
-let eq_constructor_payload (t1 t2: constructor_payload) =
+let eq_constructor_payload (t1 t2: constructor_payload) : ML bool =
   match t1, t2 with
   | VpOfNotation t1, VpOfNotation t2 -> eq_term t1 t2
   | VpArbitrary t1, VpArbitrary t2 -> eq_term t1 t2
   | VpRecord (r1, k1), VpRecord (r2, k2) ->
-    eq_tycon_record r1 r2 &&
+    eq_tycon_record r1 r2 &&&
     eq_option eq_term k1 k2
   | _ -> false
 
-let eq_tycon (t1 t2: tycon) =
+let eq_tycon (t1 t2: tycon) : ML bool =
   match t1, t2 with
   | TyconAbstract (i1, bs1, k1), TyconAbstract (i2, bs2, k2) ->
-    eq_ident i1 i2 &&
-    eq_list eq_binder bs1 bs2 &&
+    eq_ident i1 i2 &&&
+    eq_list eq_binder bs1 bs2 &&&
     eq_option eq_term k1 k2
   | TyconAbbrev (i1, bs1, k1, t1), TyconAbbrev (i2, bs2, k2, t2) ->
-    eq_ident i1 i2 &&
-    eq_list eq_binder bs1 bs2 &&
-    eq_option eq_term k1 k2 &&
+    eq_ident i1 i2 &&&
+    eq_list eq_binder bs1 bs2 &&&
+    eq_option eq_term k1 k2 &&&
     eq_term t1 t2
   | TyconRecord (i1, bs1, k1, a1, r1), TyconRecord (i2, bs2, k2, a2, r2) ->
-    eq_ident i1 i2 &&
-    eq_list eq_binder bs1 bs2 &&
-    eq_option eq_term k1 k2 &&
-    eq_list eq_term a1 a2 &&
+    eq_ident i1 i2 &&&
+    eq_list eq_binder bs1 bs2 &&&
+    eq_option eq_term k1 k2 &&&
+    eq_list eq_term a1 a2 &&&
     eq_tycon_record r1 r2
   | TyconVariant (i1, bs1, k1, cs1), TyconVariant (i2, bs2, k2, cs2) ->
-    eq_ident i1 i2 &&
-    eq_list eq_binder bs1 bs2 &&
-    eq_option eq_term k1 k2 &&
+    eq_ident i1 i2 &&&
+    eq_list eq_binder bs1 bs2 &&&
+    eq_option eq_term k1 k2 &&&
     eq_list (fun (i1, o1, a1) (i2, o2, a2) ->
-      eq_ident i1 i2 &&
-      eq_option eq_constructor_payload o1 o2 &&
+      eq_ident i1 i2 &&&
+      eq_option eq_constructor_payload o1 o2 &&&
       eq_list eq_term a1 a2) cs1 cs2
   | _ -> false
 
 let eq_lid = Ident.lid_equals
 
-let eq_lift (t1 t2: lift) =
-  eq_lid t1.msource t2.msource &&
-  eq_lid t1.mdest t2.mdest &&
+let eq_lift (t1 t2: lift) : ML bool =
+  eq_lid t1.msource t2.msource &&&
+  eq_lid t1.mdest t2.mdest &&&
   (match t1.lift_op, t2.lift_op with
   | NonReifiableLift t1, NonReifiableLift t2 -> eq_term t1 t2
   | ReifiableLift (t1, t2), ReifiableLift (t3, t4) ->
-    eq_term t1 t3 &&
+    eq_term t1 t3 &&&
     eq_term t2 t4
   | LiftForFree t1, LiftForFree t2 -> eq_term t1 t2
   | _ -> false)
 
 
-let eq_pragma (t1 t2: pragma) =
+let eq_pragma (t1 t2: pragma) : ML bool =
   match t1, t2 with
   | ShowOptions, ShowOptions -> true
   | SetOptions s1, SetOptions s2 -> s1 = s2
@@ -459,7 +470,7 @@ let eq_pragma (t1 t2: pragma) =
   | _ -> false
 
 
-let eq_qualifier (t1 t2: qualifier) =
+let eq_qualifier (t1 t2: qualifier) : ML bool =
   match t1, t2 with
   | Private, Private -> true
   | Noeq, Noeq -> true
@@ -480,46 +491,48 @@ let eq_qualifier (t1 t2: qualifier) =
   | Logic, Logic -> true
   | _ -> false
 
-let eq_qualifiers (t1 t2: qualifiers) =
+let eq_qualifiers (t1 t2: qualifiers) : ML bool =
   eq_list eq_qualifier t1 t2
 
-let eq_restriction (restriction1 restriction2: FStarC.Syntax.Syntax.restriction) =
+let eq_restriction (restriction1 restriction2: FStarC.Syntax.Syntax.restriction) : ML bool =
   let open FStarC.Syntax.Syntax in
   match restriction1, restriction2 with
   | (Unrestricted, Unrestricted) -> true
   | (AllowList l1, AllowList l2) ->
-    let eq_tuple eq_fst eq_snd (a, b) (c, d) = eq_fst a c && eq_snd b d in
-    eq_list (eq_tuple eq_ident (eq_option eq_ident)) l1 l2
+    eq_list (fun p1 p2 ->
+               let (a, b) = p1 in
+               let (c, d) = p2 in
+               eq_ident a c &&& eq_option eq_ident b d) l1 l2
   | _ -> false
 
-let rec eq_decl' (d1 d2:decl') : bool =
+let rec eq_decl' (d1 d2:decl') : ML bool =
   //generate the cases of this comparison starting with TopLevelModule
   match d1, d2 with
   | TopLevelModule lid1, TopLevelModule lid2 ->
     eq_lid lid1 lid2
   | Open (lid1, restriction1), Open (lid2, restriction2) ->
-    eq_lid lid1 lid2 &&
+    eq_lid lid1 lid2 &&&
     eq_restriction restriction1 restriction2
   | Friend lid1, Friend lid2 ->
     eq_lid lid1 lid2
   | Include (lid1, restriction1), Include (lid2, restriction2) ->
-    eq_lid lid1 lid2 &&
+    eq_lid lid1 lid2 &&&
     eq_restriction restriction1 restriction2
   | ModuleAbbrev (i1, lid1), ModuleAbbrev (i2, lid2) ->
-    eq_ident i1 i2 &&
+    eq_ident i1 i2 &&&
     eq_lid lid1 lid2
   | TopLevelLet (lq1, pats1), TopLevelLet (lq2, pats2) ->
-    lq1=lq2 &&
-    eq_list (fun (p1, t1) (p2, t2) -> eq_pattern p1 p2 && eq_term t1 t2) pats1 pats2
+    lq1=lq2 &&&
+    eq_list (fun (p1, t1) (p2, t2) -> eq_pattern p1 p2 &&& eq_term t1 t2) pats1 pats2
   | Tycon (b1, b2, tcs1), Tycon (b3, b4, tcs2) ->
-    b1 = b3 &&
-    b2 = b4 &&
+    b1 = b3 &&&
+    b2 = b4 &&&
     eq_list eq_tycon tcs1 tcs2
   | Val (i1, t1), Val (i2, t2) ->
-    eq_ident i1 i2 &&
+    eq_ident i1 i2 &&&
     eq_term t1 t2
   | Exception (i1, t1), Exception (i2, t2) ->
-    eq_ident i1 i2 &&
+    eq_ident i1 i2 &&&
     eq_option eq_term t1 t2
   | NewEffect ed1, NewEffect ed2 ->
     eq_effect_decl ed1 ed2
@@ -528,46 +541,46 @@ let rec eq_decl' (d1 d2:decl') : bool =
   | SubEffect l1, SubEffect l2 ->
     eq_lift l1 l2
   | Polymonadic_bind (lid1, lid2, lid3, t1), Polymonadic_bind (lid4, lid5, lid6, t2) ->
-    eq_lid lid1 lid4 &&
-    eq_lid lid2 lid5 &&
-    eq_lid lid3 lid6 &&
+    eq_lid lid1 lid4 &&&
+    eq_lid lid2 lid5 &&&
+    eq_lid lid3 lid6 &&&
     eq_term t1 t2
   | Polymonadic_subcomp (lid1, lid2, t1), Polymonadic_subcomp (lid3, lid4, t2) ->
-    eq_lid lid1 lid3 &&
-    eq_lid lid2 lid4 &&
+    eq_lid lid1 lid3 &&&
+    eq_lid lid2 lid4 &&&
     eq_term t1 t2
   | Pragma p1, Pragma p2 ->
     eq_pragma p1 p2
   | Assume (i1, t1), Assume (i2, t2) ->
-    eq_ident i1 i2 &&
+    eq_ident i1 i2 &&&
     eq_term t1 t2
   | Splice (is_typed1, is1, t1), Splice (is_typed2, is2, t2) ->
-    is_typed1 = is_typed2 &&
-    eq_list eq_ident is1 is2 &&
+    is_typed1 = is_typed2 &&&
+    eq_list eq_ident is1 is2 &&&
     eq_term t1 t2
   | DeclSyntaxExtension (s1, t1, _, _), DeclSyntaxExtension (s2, t2, _, _) ->
-    s1 = s2 && t1 = t2
+    s1 = s2 &&& t1 = t2
   | UseLangDecls p1, UseLangDecls p2 ->
     p1 = p2
   | DeclToBeDesugared tbs1, DeclToBeDesugared tbs2 ->
-    tbs1.lang_name = tbs2.lang_name &&
+    tbs1.lang_name = tbs2.lang_name &&&
     tbs1.eq tbs1.blob tbs2.blob
   | _ -> false
 
-and eq_effect_decl (t1 t2: effect_decl) =
+and eq_effect_decl (t1 t2: effect_decl) : ML bool =
   match t1, t2 with
   | DefineEffect (i1, bs1, t1, ds1), DefineEffect (i2, bs2, t2, ds2) ->
-    eq_ident i1 i2 &&
-    eq_list eq_binder bs1 bs2 &&
-    eq_term t1 t2 &&
+    eq_ident i1 i2 &&&
+    eq_list eq_binder bs1 bs2 &&&
+    eq_term t1 t2 &&&
     eq_list eq_decl ds1 ds2
   | RedefineEffect (i1, bs1, t1), RedefineEffect (i2, bs2, t2) ->
-    eq_ident i1 i2 &&
-    eq_list eq_binder bs1 bs2 &&
+    eq_ident i1 i2 &&&
+    eq_list eq_binder bs1 bs2 &&&
     eq_term t1 t2
   | _ -> false
 
-and eq_decl (d1 d2:decl) : bool =
-  eq_decl' d1.d d2.d &&
-  eq_list eq_qualifier d1.quals d2.quals &&
+and eq_decl (d1 d2:decl) : ML bool =
+  eq_decl' d1.d d2.d &&&
+  eq_list eq_qualifier d1.quals d2.quals &&&
   eq_list eq_term d1.attrs d2.attrs
