src/tactics/FStarC.Tactics.CtrlRewrite.fst
@@ -15,7 +15,6 @@
 *)
 
 module FStarC.Tactics.CtrlRewrite
-#push-options "--MLish --MLish_effect FStarC.Effect"
 
 open FStarC
 open FStarC.Effect
@@ -49,7 +48,7 @@ let __do_rewrite
     (rewriter : rewriter_ty)
     (env : env)
     (tm : term)
-  : tac term
+  : ML (tac term)
 =
   (*
    * We skip certain terms. In particular if the term is a constant
@@ -155,13 +154,13 @@ let do_rewrite
     (rewriter : rewriter_ty)
     (env : env)
     (tm : term)
-  : tac term
+  : ML (tac term)
   = match! catch (__do_rewrite g0 rewriter env tm) with
     | Inl SKIP -> return tm
     | Inl e -> traise e
     | Inr tm' -> return tm'
 
-type ctac 'a = 'a -> tac ('a & ctrl_flag)
+type ctac 'a = 'a -> ML (tac ('a & ctrl_flag))
 
 (* Transform a value x with c1, and continue with c2 if needed *)
 let seq_ctac (c1 : ctac 'a) (c2 : ctac 'a)
@@ -222,7 +221,7 @@ let maybe_rewrite
     (rewriter   : rewriter_ty)
     (env : env)
     (tm : term)
-  : tac (term & ctrl_flag)
+  : ML (tac (term & ctrl_flag))
   = let! (rw, ctrl_flag) = controller tm in
     let! tm' = 
          if rw
@@ -238,7 +237,7 @@ let rec ctrl_fold_env
     (rewriter : rewriter_ty)
     (env : env)
     (tm : term)
-  : tac (term & ctrl_flag)
+  : ML (tac (term & ctrl_flag))
   = let recurse tm =
       ctrl_fold_env g0 d controller rewriter env tm
     in
@@ -251,8 +250,8 @@ let rec ctrl_fold_env
       seq_ctac (on_subterms g0 d controller rewriter env)
                (maybe_rewrite g0 controller rewriter env) tm
 
-and recurse_option_residual_comp (env:env) (retyping_subst:list subst_elt) (rc_opt:option residual_comp) recurse
-  : tac (option residual_comp & ctrl_flag)
+and recurse_option_residual_comp (env:env) (retyping_subst:list subst_elt) (rc_opt:option residual_comp) (recurse: Env.env -> term -> ML (tac (term & ctrl_flag)))
+  : ML (tac (option residual_comp & ctrl_flag))
   = // return (None, Continue)
     match rc_opt with
     | None -> return (None, Continue)
@@ -271,7 +270,7 @@ and on_subterms
     (rewriter : rewriter_ty)
     (env : env)
     (tm : term)
-  : tac (term & ctrl_flag)
+  : ML (tac (term & ctrl_flag))
   = let recurse env tm = ctrl_fold_env g0 d controller rewriter env tm in
     let rr = recurse env in (* recurse on current env *)
 
@@ -282,7 +281,10 @@ and on_subterms
     // The retyping_subst is an identity substitution that replaces the bound vars
     // in the term with their new variants tagged with the rewritten bv sorts
     //
-    let rec descend_binders orig accum_binders retyping_subst accum_flag env bs t k rebuild =
+    let rec descend_binders orig accum_binders retyping_subst accum_flag env bs t k
+      (rebuild: list binder -> term -> option residual_comp -> ML term')
+      : ML (tac (term' & ctrl_flag))
+      =
       match bs with
       | [] ->
         let t = SS.subst retyping_subst t in
@@ -314,7 +316,7 @@ and on_subterms
           let retyping_subst = NT(bv, bv_to_name bv) :: retyping_subst in
           descend_binders orig (b::accum_binders) retyping_subst (par_combine (accum_flag, flag)) env bs t k rebuild
     in
-    let go () : tac (term' & ctrl_flag) =
+    let go () : ML (tac (term' & ctrl_flag)) =
       let tm = SS.compress tm in
       match tm.n with
       (* Run on hd and args in parallel *)
@@ -360,7 +362,7 @@ and on_subterms
        * and do not go into patterns.
        * also ignoring the return annotations *)
       | Tm_match {scrutinee=hd; ret_opt=asc_opt; brs; rc_opt=lopt} ->
-        let c_branch (br:S.branch) : tac (S.branch & ctrl_flag) =
+        let c_branch (br:S.branch) : ML (tac (S.branch & ctrl_flag)) =
           let (pat, w, e) = SS.open_branch br in
           let bvs = S.pat_bvs pat in
           let! e, flag = recurse (Env.push_bvs env bvs) e in
@@ -389,7 +391,7 @@ and on_subterms
       (* Descend, in parallel, in *every* definiens and the body.
        * Again body is properly opened, and we don't go into types. *)
      | Tm_let {lbs=(true, lbs); body=e} ->
-       let c_lb (lb:S.letbinding) : tac (S.letbinding & ctrl_flag) =
+       let c_lb (lb:S.letbinding) : ML (tac (S.letbinding & ctrl_flag)) =
          let! (def, flag) = rr lb.lbdef in
          return ({lb with lbdef = def }, flag)
        in
@@ -423,7 +425,7 @@ let do_ctrl_rewrite
     (rewriter   : rewriter_ty)
     (env : env)
     (tm : term)
-  : tac term
+  : ML (tac term)
   = let! tm', _ = ctrl_fold_env g0 dir controller rewriter env tm in
     return tm'
 
@@ -431,7 +433,7 @@ let ctrl_rewrite
     (dir : direction)
     (controller : controller_ty)
     (rewriter   : rewriter_ty)
-  : tac unit
+  : ML (tac unit)
   = wrap_err "ctrl_rewrite" <| (
     let! ps = get in
     let g, gs = match ps.goals with
