src/syntax/FStarC.Syntax.Visit.fst
@@ -1,5 +1,4 @@
 module FStarC.Syntax.Visit
-#push-options "--MLish --MLish_effect FStarC.Effect"
 
 open FStarC.Effect
 open FStarC.List
@@ -18,11 +17,11 @@ instance _ : monad id = {
 
 let (<<) f g = fun x -> f (g x)
 
-let visit_term pq vt t =
-  I?.run (visitM_term pq (I << vt) t)
+let visit_term pq vt t : ML _ =
+  I?.run (visitM_term pq (fun x -> I (vt x)) t)
 
-let visit_term_univs pq vt vu t =
-  I?.run (visitM_term_univs pq (I << vt) (I << vu) t)
+let visit_term_univs pq vt vu t : ML _ =
+  I?.run (visitM_term_univs pq (fun x -> I (vt x)) (fun x -> I (vu x)) t)
 
-let visit_sigelt pq vt vu se =
-  I?.run (visitM_sigelt pq (I << vt) (I << vu) se)
+let visit_sigelt pq vt vu se : ML _ =
+  I?.run (visitM_sigelt pq (fun x -> I (vt x)) (fun x -> I (vu x)) se)
