src/syntax/FStarC.Syntax.VisitM.fsti
@@ -1,6 +1,6 @@
 module FStarC.Syntax.VisitM
-#push-options "--MLish --MLish_effect FStarC.Effect"
 
+open FStarC.Effect
 open FStarC.Syntax.Syntax
 open FStarC.Class.Monad
 
@@ -8,25 +8,25 @@ open FStarC.Class.Monad
 // hopefully allowing the user to choose whether we open/close or not,
 // and know the binding depth at each point.
 
-val visitM_term
-  (#m:_) {| monad m |}
-  (proc_quotes : bool)
-  (v : term -> m term)
-  (t : term)
-  : m term
-
 val visitM_term_univs
   (#m:_) {| monad m |}
   (proc_quotes : bool)
-  (vt : term -> m term)
-  (vu : universe -> m universe)
+  (vt : term -> ML (m term))
+  (vu : universe -> ML (m universe))
   (t : term)
-  : m term
+  : ML (m term)
+
+val visitM_term
+  (#m:_) {| monad m |}
+  (proc_quotes : bool)
+  (v : term -> ML (m term))
+  (t : term)
+  : ML (m term)
 
 val visitM_sigelt
   (#m:_) {| monad m |}
   (proc_quotes : bool)
-  (vt : term -> m term)
-  (vu : universe -> m universe)
+  (vt : term -> ML (m term))
+  (vu : universe -> ML (m universe))
   (t : sigelt)
-  : m sigelt
+  : ML (m sigelt)
