src/typechecker/FStarC.TypeChecker.Quals.fsti
@@ -15,9 +15,9 @@
 *)
 
 module FStarC.TypeChecker.Quals
-#push-options "--MLish --MLish_effect FStarC.Effect"
 
 open FStarC
+open FStarC.Effect
 open FStarC.Syntax.Syntax
 open FStarC.TypeChecker.Env
   
@@ -33,5 +33,5 @@ Currently, the only things that must be checked after the function is typechecke
 - The instance attribute for typeclasses
 *)
 
-val check_sigelt_quals_pre  : env -> sigelt -> unit
-val check_sigelt_quals_post : env -> sigelt -> unit
+val check_sigelt_quals_pre  : env -> sigelt -> ML unit
+val check_sigelt_quals_post : env -> sigelt -> ML unit
